Source/DafnyRuntime/DafnyRuntimeDafny/src/array.dfy
@@ -9,6 +9,7 @@ module {:options "/functionSyntax:4"} Arrays {
   import opened Frames
   import opened Math
 
+  //
   // We use this instead of the built-in Dafny array<T> type for two reasons:
   // 
   // 1. Every element of an array<T> must be initialized.
@@ -18,11 +19,12 @@ module {:options "/functionSyntax:4"} Arrays {
   //    that could be compiled to efficient enough code instead
   //    (i.e. the Unset constructor below could be marked ghost):
   //    https://github.com/dafny-lang/rfcs/pull/11
+  //
   // 2. The array<T> type does not support any bulk-assignment
   //    operations, which are important to optimize as much as possible
   //    in this performance-sensitive code.
   //    See https://github.com/dafny-lang/dafny/issues/2447.
-  
+  //
   datatype ArrayCell<T> = Set(value: T) | Unset
 
   trait {:extern} Array<T> extends Validatable {
